DBM_Operations_Impl.thy
@@ -4,6 +4,8 @@ theory DBM_Operations_Impl
 
 begin
 
+no_notation infinity ("\<infinity>")
+
 chapter \<open>Implementation of DBM Operations\<close>
 
 section \<open>Misc\<close>
